\input{preamble.tex}
\input{environments.tex}
\input{definitions.tex}

\externaldocument{../set-theory/set-theory}

\begin{document}

\title{Discrete Mathematics}
\author{Daniel Gonzalez Cedre}
\date{University of Notre Dame \\ Spring of 2023}
\maketitle

\setcounter{chapter}{3}
\chapter{Mathematical Induction}

\section{Weak Induction}

\begin{theorem}[\(\N\) is Well-Ordered]\label{thm:lep}
    \vspace{-\parskip}
    \[
        \pn*{\forall A \subseteq \N}\pn*{A \neq \emptyset \implies \pn*{\exists a \in A}\pn*{\forall b \in A}\pn*{a \leq b}}
    \]
    This says that every nonempty subset of \(\N\) has a least element
    (according to the \(\leq\) order defined on \(\N\)).
\end{theorem}
\begin{proof}
    This proof is left as an exercise.
\end{proof}

\begin{theorem}[Weak Induction]
    If \(\varphi(\cdot)\) is a {\wff}, then
    \[
        \pn*{\forall n \in \N}\pn*{\varphi(n)}
        ~\iff~ \varphi(0) \meet \pn*{\forall k \in \N}\pn*{\varphi(k) \implies \varphi(k + 1)}.
    \]
\end{theorem}
\begin{proof}
    There are two fragments to this proof:
    the forward (\(\implies\)) direction and the backward (\(\impliedby\)) direction.

    \begin{case}[Fragment 1 (\(\implies\))]
        Suppose that \(\pn*{\forall n \in \N}\pn*{\varphi(n)}\).
        Since \(0 \in \N\), we then obviously have \(\varphi(0)\).
        Now, let \(k \in \N\) and assume \(\varphi(k)\).
        Since \(k + 1 \in \N\), we know from our initial assumption that \(\varphi(k + 1)\).
        Thus, we have \(\pn*{\forall k \in \N}\pn*{\varphi(k) \implies \varphi(k + 1)}\),
        and we have reached both of our desired conclusions.
    \end{case}

    \begin{case}[Fragment 2 (\(\impliedby\))]
        Assume \(\varphi(0)\) and \(\pn*{\forall k \in \N}\pn*{\varphi(k) \implies \varphi(k + 1)}\).
        Towards a contradiction,
        suppose that there is some \(n \in \N\) such that \(\neg \varphi(a)\).
        Consider \(A \defn \set*{x \in \N \suchthat \neg \varphi(x)}\),
        which we clearly know exists by \autoref{ax:separation}.
        We know that \(n \in A\) because we assumed that \(\neg \varphi(n)\),
        which implies that \(A \neq \emptyset\).
        Then, we can use \autoref{thm:lep} to conclude that there is a minimal element \(a\) in \(A\).

        Since we know that \(\varphi(0)\), it follows that \(a \neq 0\), so \(a\) must be a successor number.
        This means there is a \(b \in \N\) such that \(b + 1 = a\).

        If \(b \in A\), then that would mean that \(a \leq b\) since \(a\) is minimal in \(A\).
        However, we know that \(b < b + 1 = a\), so we would then have \(a \leq b < a\). \contradiction\\
        Therefore, \(b \not \in A\).

        % Since we assumed \(\neg \varphi(n)\), we know \(n \in A\) by definition,
        % showing us that \(A \neq \emptyset\).
        % Since we assumed \(\varphi(0)\), we know that \(0 \not \in A\) by definition,
    \end{case}
\end{proof}

Let's practice induction by proving the following theorem.
\newpage
\begin{theorem}[Gaussian Summation Formula]\label{thm:gaussiansum}
    \[
        \pn*{\forall n \in \N}\pn*{\sum_{i = 0}^{n}i = \frac{n(n + 1)}{2}}.
    \]
\end{theorem}
\begin{proof}
    We will prove the claim by induction on \(n \in \N\).

    \begin{case}[Base Case]
        Observe that \(\sum_{i = 0}^{0}i = 0 = \frac{0*(0 + 1)}{2}\).
        Therefore, the statement is satisfied at \(0\).
    \end{case}

    \begin{case}[Inductive Step]
        Let \(k \in \N\) and assume \(\sum_{i = 0}^{k}i = \frac{k(k + 1)}{2}\)
        (this is our \emph{inductive hypothesis}).
        Now, observe
        \begin{alignat*}{2}
            \sum_{i = 0}^{k + 1}i &= \pn*{\sum_{i = 0}^{k}i} + (k + 1) &&\text{ by definition}\\
                                  &= \pn*{\frac{k(k + 1)}{2}} + (k + 1)~~~~&&\text{ by the \emph{inductive hypothesis}}\\
                                  &= (k + 1)\pn*{\frac{k}{2} + 1} &&\text{ by factoring out } (k + 1)\\
                                  &= \frac{(k + 1)(k + 2)}{2} &&\text{ because } \frac{k}{2} + 1 = \frac{k}{2} + \frac{2}{2} = \frac{k + 2}{2}.
        \end{alignat*}
        Thus, we have that \(\sum_{i = 0}^{k + 1}i = \frac{(k + 1)(k + 2)}{2}\), as desired.
    \end{case}

    Therefore, we can conclude that \(\pn*{\forall n \in \N}\pn*{\sum_{i = 0}^{n}i = \frac{n(n + 1)}{2}}\).
\end{proof}

\end{document}
