\input{preamble.tex}
\input{environments.tex}
\input{definitions.tex}

\externaldocument{../first-order-logic/first-order-logic}

\begin{document}

\title{Discrete Mathematics}
\author{Daniel Gonzalez Cedre}
\date{University of Notre Dame \\ Spring of 2023}
\maketitle

\setcounter{chapter}{0}
\chapter{Propositional Logic}\label{chap:propositional}

\section{Propositions \& Connectives}

\begin{definition}[Proposition]
    A \emph{proposition} is a statement
    that has \emph{one and only one} consistent truth value.
\end{definition}

\begin{definition}[Satisfiability]
    A propositional expression $\varphi$ consisting the propositional variables $p_1, \dots p_n$ is \emph{satisfiable}
    \iffbydefn there exists an assignment of truth values to $p_1, \dots p_n$ that results in $\varphi$ being equivalent to $\top$.
\end{definition}


\begin{definition}[Negation]
    ~
    \begin{center}
        \begin{minipage}[t]{.55\linewidth}
            Given a proposition $p$, the \emph{negation} of $p$
            is denoted $\neg p$ and can be defined by the following truth table:
            \begin{table}[H]
                \centering
                \label{tab:not}
                \begin{tabular}{|Cc||Cc|} \hline
                    \thead{$p$} & \thead{$\neg p$} \\ \hline
                    \thead{$\top$} & \cellcolor{red!30!white}{\thead{$\bot$}} \\
                    \thead{$\bot$} & \cellcolor{green!30!white}{\thead{$\top$}} \\ \hline
                \end{tabular}
            \end{table}
        \end{minipage}%
        \begin{minipage}[t]{.05\linewidth}
            ~
        \end{minipage}%
        \begin{minipage}[t]{.4\linewidth}
            Some possible readings of $\neg p$:\\
            \begin{list}{$\cdot$}{}
                \item
                    Not $p$.
                \item
                    $p$ does not hold.
                \item
                    It is not the case that $p$.
                \item
                    We do not have that $p$.
            \end{list}
        \end{minipage}
    \end{center}
\end{definition}

\begin{definition}[Conjunction]
    ~
    \begin{center}
        \begin{minipage}[t]{.55\linewidth}
            Given two propositions $p$ and $q$, the \emph{conjunction} of $p$ with $q$
            is denoted $p \meet q$ and can be defined by the following truth table:
            \begin{table}[H]
                \centering
                \label{tab:and}
                \begin{tabular}{|CcCc||Cc|} \hline
                    \thead{$p$} & \thead{$q$} & \thead{$p \meet q$} \\ \hline
                    \thead{$\top$} & \thead{$\top$} & \cellcolor{green!30!white}{\thead{$\top$}} \\
                    \thead{$\top$} & \thead{$\bot$} & \cellcolor{red!30!white}{\thead{$\bot$}} \\
                    \thead{$\bot$} & \thead{$\top$} & \cellcolor{red!30!white}{\thead{$\bot$}} \\
                    \thead{$\bot$} & \thead{$\bot$} & \cellcolor{red!30!white}{\thead{$\bot$}} \\ \hline
                \end{tabular}
            \end{table}
        \end{minipage}%
        \begin{minipage}[t]{.05\linewidth}
            ~
        \end{minipage}%
        \begin{minipage}[t]{.4\linewidth}
            Some possible readings of $p \meet q$:\\
            \begin{list}{$\cdot$}{}
                \item
                    $p$, and $q$.
                \item
                    $p$, but $q$.
                \item
                    $p$; also, $q$.
                \item
                    $p$; further, $q$.
                \item
                    In addition to $p$, we also have $q$.
            \end{list}
        \end{minipage}
    \end{center}
\end{definition}


\begin{definition}[Disjunction]
    ~
    \begin{center}
        \begin{minipage}[t]{.55\linewidth}
            Given two propositions $p$ and $q$, the \emph{disjunction} of $p$ with $q$
            is denoted $p \join q$ and can be defined by the following truth table:
            \begin{table}[H]
                \centering
                \label{tab:or}
                \begin{tabular}{|CcCc||Cc|} \hline
                    \thead{$p$} & \thead{$q$} & \thead{$p \join q$} \\ \hline
                    \thead{$\top$} & \thead{$\top$} & \cellcolor{green!30!white}{\thead{$\top$}} \\
                    \thead{$\top$} & \thead{$\bot$} & \cellcolor{green!30!white}{\thead{$\top$}} \\
                    \thead{$\bot$} & \thead{$\top$} & \cellcolor{green!30!white}{\thead{$\top$}} \\
                    \thead{$\bot$} & \thead{$\bot$} & \cellcolor{red!30!white}{\thead{$\bot$}} \\ \hline
                \end{tabular}
            \end{table}
        \end{minipage}%
        \begin{minipage}[t]{.05\linewidth}
            ~
        \end{minipage}%
        \begin{minipage}[t]{.4\linewidth}
            Some possible readings of $p \join q$:\\
            \begin{list}{$\cdot$}{}
                \item
                    $p$, or $q$.
                \item
                    Either $p$, or $q$.
            \end{list}
        \end{minipage}
    \end{center}
\end{definition}

\begin{definition}[Material Implication]
    ~
    \begin{center}
        \begin{minipage}[t]{.55\linewidth}
            Given two propositions $p$ and $q$,
            the \emph{conditional} formed by assuming $p$ and concluding $q$
            is denoted $p \rightarrow q$ and can be defined by the following truth table:
            \begin{table}[H]
                \centering
                \label{tab:implies}
                \begin{tabular}{|CcCc||Cc|} \hline
                    \thead{$p$} & \thead{$q$} & \thead{$p \rightarrow q$} \\ \hline
                    \thead{$\top$} & \thead{$\top$} & \cellcolor{green!30!white}{\thead{$\top$}} \\
                    \thead{$\top$} & \thead{$\bot$} & \cellcolor{red!30!white}{\thead{$\bot$}} \\
                    \thead{$\bot$} & \thead{$\top$} & \cellcolor{green!30!white}{\thead{$\top$}} \\
                    \thead{$\bot$} & \thead{$\bot$} & \cellcolor{green!30!white}{\thead{$\top$}} \\ \hline
                \end{tabular}
            \end{table}
        \end{minipage}%
        \begin{minipage}[t]{.05\linewidth}
            ~
        \end{minipage}%
        \begin{minipage}[t]{.4\linewidth}
            Some possible readings of $p \rightarrow q$:\\
            \begin{list}{$\cdot$}{}
                \item
                    If $p$, then $q$.
                \item
                    $p$ implies $q$.
                \item
                    $q$ is conditioned on $p$.
                \item
                    $q$ only if $p$.
                \item
                    $p$ is sufficient for $q$.
                \item
                    $q$ is necessary for $p$.
                \item
                    $q$ unless not $p$.
                \item
                    $q$ or not $p$.
            \end{list}
        \end{minipage}
    \end{center}
\end{definition}

\begin{definition}[Material Equivalence]
    ~
    \begin{center}
        \begin{minipage}[t]{.55\linewidth}
            Given two propositions $p$ and $q$, the \emph{biconditional} formed by $p$ and $q$
            is denoted $p \leftrightarrow q$ and can be defined by the following truth table:
            \begin{table}[H]
                \centering
                \label{tab:iff}
                \begin{tabular}{|CcCc||Cc|} \hline
                    \thead{$p$} & \thead{$q$} & \thead{$p \leftrightarrow q$} \\ \hline
                    \thead{$\top$} & \thead{$\top$} & \cellcolor{green!30!white}{\thead{$\top$}} \\
                    \thead{$\top$} & \thead{$\bot$} & \cellcolor{red!30!white}{\thead{$\bot$}} \\
                    \thead{$\bot$} & \thead{$\top$} & \cellcolor{red!30!white}{\thead{$\bot$}} \\
                    \thead{$\bot$} & \thead{$\bot$} & \cellcolor{green!30!white}{\thead{$\top$}} \\ \hline
                \end{tabular}
            \end{table}
        \end{minipage}%
        \begin{minipage}[t]{.05\linewidth}
            ~
        \end{minipage}%
        \begin{minipage}[t]{.4\linewidth}
            Some possible readings of $p \leftrightarrow q$:\\
            \begin{list}{$\cdot$}
                \item
                    $p$ if and only if $q$.
                \item
                    $p$ is necessary and sufficient for $q$.
                \item
                    $q$ is necessary and sufficient for $p$.
            \end{list}
        \end{minipage}
    \end{center}
\end{definition}

\begin{definition}[Equivalence]
    If we have two expressions $\varphi$ and $\psi$ in our formal language,
    consisting of some number of (possibly shared) propositional variables, connected together by logical connectives,
    then with the notation $\varphi \iff \psi$ we say that $\varphi$ is equivalent to $\psi$
    \iffbydefn every assignment of truth values to the propositional variables of $\varphi$ and $\psi$ results
    in the same truth value for the two expressions.
\end{definition}
\begin{example}
    Consider the two expressions $\varphi \defn p \rightarrow q$ and $\psi \defn \neg p \join q$.
    We can see that $\varphi$ has two propositional variables: $p$ and $q$.
    $\psi$ also has two propositional variables: the same $p$ and the same $q$.
    If we construct the truth table for these two expressions,
    we will see that every assignment of truth values to $p$ and $q$ will result in $p \rightarrow q$ and $\neg p \join q$
    having the same truth value.

    \begin{table}[H]
        \centering
        \begin{tabular}{|CcCc||CcCc|} \hline
            \thead{$p$} & \thead{$q$} & \thead{$p \rightarrow q$} & \thead{$\neg p \join q$}\\ \hline
            \thead{$\top$} & \thead{$\top$} & \cellcolor{green!30!white}{\thead{$\top$}} & \cellcolor{green!30!white}{$\top$}\\
            \thead{$\top$} & \thead{$\bot$} & \cellcolor{red!30!white}{\thead{$\bot$}} & \cellcolor{red!30!white}{\thead{$\bot$}}\\
            \thead{$\bot$} & \thead{$\top$} & \cellcolor{green!30!white}{\thead{$\top$}} & \cellcolor{green!30!white}{\thead{$\top$}} \\
            \thead{$\bot$} & \thead{$\bot$} & \cellcolor{green!30!white}{\thead{$\top$}} & \cellcolor{green!30!white}{\thead{$\top$}} \\ \hline
        \end{tabular}
    \end{table}
\end{example}

\newpage

\section{Boolean Algebras}

\begin{definition}[Boolean Algebra]\label{def:boolean}
    A \emph{Boolean algebra} is a collection of \emph{terms} $B$
    with two distinguished (and distinct) terms called $\top$ and $\bot$,
    along with a unary operation called $\neg$ and two binary operations called $\meet$ and $\join$,
    such that the following statements are true for any terms $p, q, r$ in $B$:

    \begin{table}[H]
        \centering
        \label{tab:boole}
        \begin{tabular}{|Cc|Cc|} \hline
            \multicolumn{2}{|c|}{\thead{Axioms of a Boolean Algebra}} \\\hline
            \thead{Identity} & \thead{$p \meet \top \iff p$ \\ $p \join \bot \iff p$} \\ \hline
            \thead{Complement \\ (\aka Negation)} & \thead{$p \meet \neg p \iff \bot$ \\ $p \join \neg p \iff \top$} \\ \hline
            \thead{Commutativity} & \thead{$p \meet q \iff q \meet p$ \\ $p \join q \iff q \join p$} \\ \hline
            \thead{Associativity} & \thead{$p \meet (q \meet r) \iff (p \meet q) \meet r$ \\ $p \join (q \join r) \iff (p \join q) \join r$} \\ \hline
            \thead{Distributive Laws} & \thead{$p \conjunct (q \disjunct r) \iff (p \conjunct q) \disjunct (p \conjunct r)$ \\ $p \disjunct (q \conjunct r) \iff (p \disjunct q) \conjunct (p \disjunct r)$} \\ \hline
        \end{tabular}
    \end{table}

    This kind of structure is also referred to as a \emph{complemented, distributive lattice}.
    Since we are establishing the algebra of \emph{propositions},
    our terms consist only of $\top$ and $\bot$.

    However, since none of these axioms tell us how to use the (very useful) symbols
    $\rightarrow$ and $\leftrightarrow$, we need two additional axioms that will turn our Boolean algebra
    into an example of a \emph{Heyting algebra}:

    \begin{table}[H]
        \centering
        \label{tab:heyting}
        \begin{tabular}{|Cc|Cc|} \hline
            \multicolumn{2}{|c|}{\thead{Heyting Axioms}} \\\hline
            \thead{Conditional Disintegration}   & \thead{$p \rightarrow q \iff \neg p \join q$} \\ \hline
            \thead{Biconditional Disintegration} & \thead{$p \leftrightarrow q \iff (p \rightarrow q) \meet (q \rightarrow p)$} \\ \hline
        \end{tabular}
    \end{table}

    By referring to the truth tables,
    it should be easy to see that these axioms are \emph{truth preserving} transformations,
    meaning that taking an expression like $p \meet (q \rightarrow r)$
    and applying an axiom like Identity to it
    does not change the truth value of the resulting expression $(p \meet \top) \meet (q \rightarrow r)$.
    For this reason, these are sometimes referred to as \emph{equivalence laws} and many treatments of this subject
    \emph{prove} these laws by referring to the truth tables.

    For our purposes, we don't need to refer to the truth tables at all.
    The truth tables were a nice, intuitive, and compact way of defining the logical connectives,
    but we could just as easily have defined them by assuming that all of the axioms are true,
    without ever writing down a truth table.
    This provides a more \emph{algebraic} approach to the study of logic,
    which is more in-line with the way logic is used to actually prove theorems in mathematics.

    As such, while the while the truth tables provided a nice way of defining the logical connectives,
    we will be taking the algebraic approach by \emph{assuming the axioms} of a Boolean algebra
    are true about our propositional logic
    and using them to prove theorems about our logical system.
\end{definition}

\begin{definition}[Tautology]
    We say a proposition $\varphi$ is a \emph{tautology}
    \iffbydefn we have that $\varphi \iff \top$.
\end{definition}
\begin{definition}[Contradiction]
    We say a proposition $\varphi$ is a \emph{contradiction}
    \iffbydefn we have that $\varphi \iff \bot$.
\end{definition}
\begin{example}
    $p \join \neg p$ is a tautology, and $p \meet \neg p$ is a contradiction.
\end{example}

\begin{theorem}[Uniqueness of Complements]\label{thm:unique}
    Let $p$ be a term in a Boolean algebra $(B, \neg, \meet, \join)$.
    Suppose there were two terms $x$ and $y$ in the Boolean algebra such that
    \begin{center}
        \begin{minipage}{.2\linewidth}
            \begin{align*}
                p \meet x &\iff \bot,\\
                p \join x &\iff \top,
            \end{align*}
        \end{minipage}%
        \begin{minipage}{.2\linewidth}
            \begin{align*}
                p \meet y &\iff \bot,\\
                p \join y &\iff \top,
            \end{align*}
        \end{minipage}
    \end{center}
    meaning that $x$ and $y$ act like negations for $p$.
    Then, we have $x \iff y$.
\end{theorem}
\begin{proof}
    Let $(B, \neg, \meet, \join)$ be a Boolean algebra
    and consider an arbitrary term $p$ in the algebra.
    Suppose we have $x$ and $y$ satisfying the conditions given in the statement of the theorem above.
    Then, we can observe
    \begin{alignat*}{2}
        x &\iff \top \meet x ~~~~~~~~~~~~~~~~&&\text{by Identity}\\
          &\iff (p \join y) \meet x &&\text{by the assumption $p \join y \iff \top$}\\
          &\iff (p \meet x) \join (y \meet x) &&\text{by Distributivity}\\
          &\iff \bot \join (y \meet x) &&\text{by the assumption $p \meet x \iff \bot$}\\
          &\iff y \meet x &&\text{by Identity}.
    \end{alignat*}
    Similarly, we can see that
    \begin{alignat*}{2}
        y &\iff \top \meet y ~~~~~~~~~~~~~~~~&&\text{by Identity}\\
          &\iff (p \join x) \meet y &&\text{by the assumption $p \join x \iff \top$}\\
          &\iff (p \meet y) \join (x \meet y) &&\text{by Distributivity}\\
          &\iff \bot \join (x \meet y) &&\text{by the assumption $p \meet y \iff \bot$}\\
          &\iff x \meet y &&\text{by Identity}.
    \end{alignat*}
    So, from Commutativity, we can conclude that $x \iff (y \meet x) \iff (x \meet y) \iff y$.
\end{proof}

\begin{lemma}
    For every Boolean algebra $(B, \neg, \meet, \join)$, we have
    \begin{align*}
        \neg \top &\iff \bot\\
        \neg \bot &\iff \top.
    \end{align*}
\end{lemma}
\begin{proof}
    Let $(B, \neg, \meet, \join)$ be a Boolean algebra with the distinguished terms $\top$ and $\bot$.
    We will show that $\neg \top \iff \bot$ by showing that
    $\neg \top$ and $\bot$ both act like negations for $\top$.

    First, observe $\neg \top \meet \top \iff \bot$ by the Complement rule.
    Similarly, we have $\neg \top \join \top \iff \top$ by the Complement rule.
    Now, $\bot \meet \top \iff \bot$ by the Identity rule.
    Similarly, $\bot \join \top \iff \top \join \bot \iff \bot$ by the Identity rule
    (and Commutativity).
    This shows us that $\neg \top$ and $\bot$ are both negations for $\top$.
    Therefore, recalling that complements are unique by \autoref{thm:unique},
    we can conclude $\neg \top \iff \bot$.
    Showing $\neg \bot \iff \top$ is left as an exercise to the reader.
\end{proof}

\begin{theorem}[Double Negation]
    For any Boolean algebra $(B, \neg, \meet, \join)$ and any term $p$ in $B$,
    we have $\neg \neg p \iff p$.
\end{theorem}
\begin{proof}
    Let $(B, \neg, \meet, \join)$ be a Boolean algebra
    and consider an arbitrary term $p$ in the algebra.
    We want to show that $\neg \neg p \iff p$,
    which we can do by establishing that $p$ and $\neg \neg p$ are both complements of $\neg p$.
    By the Complement rule, we know $p \meet \neg p \iff \bot$ and $p \join \neg p \iff \top$,
    meaning that $p$ is the complement of $\neg p$.
    Similarly, we can see that
    $\neg p \meet \neg (\neg p) \iff \bot$ and $\neg p \join \neg (\neg p) \iff \top$,
    showing us that $\neg \neg p$ is the complement of $\neg p$.
    Since complements are unique, as seen in \autoref{thm:unique},
    and both $p$ and $\neg \neg p$ are complements of $\neg p$,
    we can conclude that $p \iff \neg \neg p$.
\end{proof}

\begin{theorem}[Idempotency]
    For every Boolean algebra $(B, \neg, \meet, \join)$ and every term $p$ in the algebra,
    we have
    \begin{align*}
        p \meet p &\iff p\\
        p \join p &\iff p.
    \end{align*}
\end{theorem}
\begin{proof}
    Let $p$ be a term in an arbitrary Boolean algebra $(B, \neg, \meet, \join)$.
    Observe

    \begin{minipage}{.45\linewidth}
        \vspace{-\parskip-\abovedisplayskip}
        \begin{alignat*}{2}
            p \meet p &\iff (p \meet p) \join \bot~~~~~~~~~~~~&&\text{by Identity}\\
                        &\iff (p \meet p) \join (p \meet \neg p) &&\text{by Complement}\\
                        &\iff p \meet (p \join \neg p) &&\text{by Distributivity}\\
                        &\iff p \meet \top &&\text{by Complement}\\
                        &\iff p &&\text{by Identity},
        \end{alignat*}
    \end{minipage}
    \hfill\vline\hfill
    \begin{minipage}{.45\linewidth}
        \vspace{-\parskip-\abovedisplayskip}
        \begin{alignat*}{2}
            p \join p &\iff (p \join p) \meet \top~~~~~~~~~~~~&&\text{by Identity}\\
                        &\iff (p \join p) \meet (p \join \neg p) &&\text{by Complement}\\
                        &\iff p \join (p \meet \neg p) &&\text{by Distributivity}\\
                        &\iff p \join \bot &&\text{by Complement}\\
                        &\iff p &&\text{by Identity}.
        \end{alignat*}
    \end{minipage}

    Therefore, $p \meet p \iff p$ and $p \join p \iff p$, as desired.
\end{proof}

% TODO
\begin{theorem}[Domination]
    For every Boolean algebra $(B, \neg, \meet, \join)$ and every term $p$ in the algebra,
    we have
    \begin{align*}
        p \meet \bot &\iff \bot\\
        p \join \top &\iff \top.
    \end{align*}
\end{theorem}
\begin{proof}
    Let $p$ be a term in an arbitrary Boolean algebra $(B, \neg, \meet, \join)$.
    Observe

    \begin{minipage}{.45\linewidth}
        \vspace{-\parskip-\abovedisplayskip}
        \begin{alignat*}{2}
            p \meet \bot &\iff p \meet (p \meet \neg p)~~~~~~~~~~~~&&\text{by Complement}\\
                            &\iff (p \meet p) \meet \neg p &&\text{by Associativity}\\
                            &\iff p \meet \neg p &&\text{by Idempotency}\\
                            &\iff \bot &&\text{by Complement},
        \end{alignat*}
    \end{minipage}
    \hfill\vline\hfill
    \begin{minipage}{.45\linewidth}
        \vspace{-\parskip-\abovedisplayskip}
        \begin{alignat*}{2}
            p \join \top &\iff p \join (p \join \neg p)~~~~~~~~~~~~&&\text{by Complement}\\
                            &\iff (p \join p) \join \neg p &&\text{by Associativity}\\
                            &\iff p \join \neg p &&\text{by Idempotency}\\
                            &\iff \top &&\text{by Complement}.
        \end{alignat*}
    \end{minipage}

    Therefore, $p \meet \bot \iff \bot$ and $p \join \top \iff \top$.
\end{proof}

\begin{theorem}[Absorption]
    For every Boolean algebra $(B, \neg, \meet, \join)$ and any two terms $p$ and $q$ in the algebra,
    we have
    \begin{align*}
        p \meet (p \join q) &\iff p\\
        p \join (p \meet q) &\iff q.
    \end{align*}
\end{theorem}
\begin{proof}
    Let $p$ and $q$ be terms in an arbitrary Boolean algebra $(B, \neg, \meet, \join)$.
    Observe

    \begin{minipage}{.45\linewidth}
        \vspace{-\parskip-\abovedisplayskip}
        \begin{alignat*}{2}
            p \meet (p \join q) &\iff (p \join \bot) \meet (p \join q)~~&&\text{by Identity}\\
                                &\iff p \join (\bot \meet q) &&\text{by Distributivity}\\
                                &\iff p \join \bot &&\text{by Domination}\\
                                &\iff p &&\text{by Identity},
        \end{alignat*}
    \end{minipage}%
    \hfill\vline\hfill
    \begin{minipage}{.45\linewidth}
        \vspace{-\parskip-\abovedisplayskip}
        \begin{alignat*}{2}
            p \join (p \meet q) &\iff (p \meet \top) \join (p \meet q)~~&&\text{by Identity}\\
                                &\iff p \meet (\top \join q) &&\text{by Distributivity}\\
                                &\iff p \meet \top &&\text{by Domination}\\
                                &\iff p &&\text{by Identity}.
        \end{alignat*}
    \end{minipage}

    Therefore, $p \meet (p \join q) \iff p$ and $p \join (p \meet q) \iff q$.
\end{proof}

\begin{theorem}[De Morgan's Laws]
    For every Boolean algebra $(B, \neg, \meet, \join)$ and any two terms $p$ and $q$ in the algebra,
    we have
    \begin{align*}
        \neg (p \meet q) &\iff \neg p \join \neg q\\
        \neg (p \join q) &\iff \neg p \meet \neg q.
    \end{align*}
\end{theorem}
\begin{proof}
    Let $p$ and $q$ be terms in an arbitrary Boolean algebra $(B, \neg, \meet, \join)$.
    Observe that
    \begin{alignat*}{2}
        (p \meet q) \meet (\neg p \join \neg q) &\iff (q \meet p) \meet (\neg p \join \neg q)~~~~~~~~~~~~&&\text{by Commutativity}\\
                                                &\iff q \meet (p \meet (\neg p \join \neg q)) &&\text{by Associativity}\\
                                                &\iff q \meet \pn*{(p \meet \neg p) \join (p \meet \neg q)} &&\text{by Distributivity}\\
                                                &\iff q \meet (\bot \join (p \meet \neg q)) &&\text{by Complement}\\
                                                &\iff q \meet (p \meet \neg q) &&\text{by Identity}\\
                                                &\iff q \meet (\neg q \meet p) &&\text{by Commutativity}\\
                                                &\iff (q \meet \neg q) \meet p &&\text{by Associativity}\\
                                                &\iff \bot \meet p &&\text{by Complement}\\
                                                &\iff \bot &&\text{by Domination}.
    \end{alignat*}

\newpage

    Further, we have
    \begin{alignat*}{2}
        (p \meet q) \join (\neg p \join \neg q) &\iff (p \meet q) \meet (\neg q \join \neg p)~~~~~~~~~~~~&&\text{by Commutativity}\\
                                                &\iff \pn*{(p \meet q) \join \neg q} \join \neg p &&\text{by Associativity}\\
                                                &\iff \pn*{(p \join \neg q) \meet (q \join \neg q)} \join \neg p &&\text{by Distributivity}\\
                                                &\iff \pn*{(p \join \neg q) \meet \top} \join \neg p &&\text{by Complement}\\
                                                &\iff (p \join \neg q) \join \neg p &&\text{by Identity}\\
                                                &\iff (\neg q \join p) \join \neg p &&\text{by Commutativity}\\
                                                &\iff \neg q \join (p \join \neg p) &&\text{by Associativity}\\
                                                &\iff \neg q \join \top &&\text{by Complement}\\
                                                &\iff \top &&\text{by Domination}.
    \end{alignat*}
    So, we can see that $\neg p \join \neg q$ is a complement for $p \meet q$.
    Since complements are unique by \autoref{thm:unique},
    we can conclude that $\neg (p \meet q) \iff \neg p \join \neg q$.

    Showing $\neg (p \join q) \iff \neg p \meet \neg q$ is left as an exercise to the reader.
\end{proof}
\end{document}
